safe

Phi_Examples/PhiEx_BinTree.c
@@ -1,0 +1,173 @@
+#include <stdbool.h>
+
+typedef int K;
+typedef int V;
+
+struct KV_pair {
+  K k;
+  V v;
+};
+
+struct BinTree {
+  struct BinTree *left;
+  struct KV_pair data;
+  struct BinTree *right;
+};
+
+struct AVL_data {
+  int height;
+  V v;
+};
+
+struct AVL_KV {
+  K k;
+  struct AVL_data v;
+};
+
+struct AVLTree {
+  struct BinTree *left;
+  struct AVL_KV data;
+  struct BinTree *right;
+};
+
+
+V lookup_bst (struct BinTree *addr, K k) {
+  K k2 = addr->data.k;
+  if (k2 == k) return addr->data.v;
+  else if (k < k2)
+    return lookup_bst (addr->left, k);
+  else
+    return lookup_bst (addr->right, k);
+}
+
+bool defined_bst (struct BinTree *addr, K k) {
+  if (addr == 0) return false;
+  K k2 = addr->data.k;
+  if (k2 == k) return true;
+  else if (k < k2)
+    return defined_bst (addr->left, k);
+  else
+    return defined_bst (addr->right, k);
+}
+
+void insert_bst (struct BinTree *addr, K k, V v) {
+  if (addr == 0) {
+    struct BinTree *ret = calloc(sizeof(struct BinTree), 1);
+    ret -> data -> k = k;
+    ret -> data -> v = v;
+    return ret;
+  } else {
+    K k2 = addr -> data -> k;
+    if (k == k2) {
+      struct BinTree *aL = insert_bst (addr -> left, k, v);
+      addr -> left = aL;
+      return addr;
+    } else {
+      struct BinTree *aL = insert_bst (addr -> right, k, v);
+      addr -> right = aL;
+      return addr;
+    }
+  }
+}
+
+int Max(int x, int y) {
+  if (x < y) return y; else return x;
+}
+
+int height_of (struct BinTree *addr) {
+  if (addr == 0)
+    return 0;
+  else
+    return addr -> data -> v -> height;
+}
+
+void maintain_i (struct BinTree *aD) {
+  struct BinTree *B = aD -> left;
+  struct BinTree *E = aD -> right;
+  int HB = height_of(B);
+  int HE = height_of(E);
+  if (HB == HE + 2) {
+    struct BinTree *A = B -> left;
+    struct BinTree *C = B -> right;
+    int HA = height_of(A);
+    int HC = height_of(C);
+    if (HC <= HA) {
+      aD -> left = C;
+      int HD2 = Max(HC, HE) + 1;
+      aD -> data -> v -> height = HD2;
+      B -> right = aD;
+      B -> data -> v -> height = Max(HA, HD2) + 1;
+      return B;
+    } else {
+      struct BinTree *CL = C -> left;
+      struct BinTree *CR = C -> right;
+      B -> right = CL;
+      int HB2 = Max(HA, height_of(CL)) + 1;
+      B -> data -> v -> height = HB2;
+      aD -> left = C -> right;
+      int HD2 = Max(HE, height_of(CR)) + 1;
+      aD -> data -> v -> height = HD2;
+      C -> left = B;
+      C -> right = aD;
+      C -> data -> v -> height = Max(HB2, HD2) + 1;
+      return C;
+    }
+  } else if (HE == HB + 2) {
+    struct BinTree *F = E -> left;
+    struct BinTree *G = E -> right;
+    int HF = height_of (F);
+    int HG = height_of (G);
+    if (HF <= HG) {
+      aD -> right = F;
+      int HD2 = Max(HB, HF) + 1;
+      aD -> data -> v -> height = HD2;
+      E -> left = aD;
+      E -> data -> v -> height = Max(HD2, HG) + 1;
+      return E;
+    } else {
+      struct BinTree *FL = F -> left;
+      struct BinTree *FR = F -> right;
+      aD -> right = FL;
+      int HD2 = Max(HB, height_of(FL)) + 1;
+      aD -> data -> v -> height = HD2;
+      E -> left = FR;
+      int HE2 = Max(height_of(FR), HG) + 1;
+      E -> data -> v -> height = HE2;
+      F -> left = aD;
+      F -> right = E;
+      F -> data -> height = Max(HD2, HE2) + 1;
+      return F;
+    }
+  } else {
+    aD -> data -> v -> height = Max(height_of(aD -> left), height_of(aD -> right)) + 1;
+    return aD;
+  }
+}
+
+void insert_avl (struct BinTree *addr, K k, V v) {
+  if (addr == 0) {
+    struct BinTree *ret = calloc(sizeof(struct BinTree), 1);
+    ret -> data -> k = k;
+    ret -> data -> v -> v = v;
+    ret -> data -> v -> height = 1;
+    return ret;
+  } else {
+    K k2 = addr -> data -> k;
+    if (k2 == k) {
+      addr -> data -> v -> v = v;
+      return addr;
+    } else {
+      if (k < k2) {
+        struct BinTree *aL = insert_avl_i (addr -> left, k, v);
+        addr -> left = aL;
+        return maintain_i(addr);
+      } else {
+        struct BinTree *aR = insert_avl_i (addr -> right, k, v);
+        addr -> right = aR;
+        return maintain_i(addr);
+      }
+    }
+  }
+}
+
+
