Phi_Semantics/PhiSem_Base.thy
@@ -6,6 +6,7 @@ section \<open>Semantics Base\<close>
 
 subsection \<open>Type Classes for Common Reasoning Strategies\<close>
 
+(*
 definition Atomic_SemTyp :: \<open>TY \<Rightarrow> bool\<close>
   where \<open>Atomic_SemTyp TY \<equiv> True\<close>
 
@@ -17,7 +18,7 @@ declare [[
   \<phi>reason_default_pattern \<open>Atomic_SemTyp ?TY\<close> \<Rightarrow> \<open>Atomic_SemTyp ?TY\<close> (100),
   \<phi>default_reasoner_group \<open>Atomic_SemTyp _\<close> : %Atomic_SemTyp (100)
 ]]
-
+*)
 
 
 end
